src/ecAlgTactic.mli
@@ -9,7 +9,7 @@ open EcAlgebra
 val is_module_loaded : EcEnv.env -> bool
 
 (* -------------------------------------------------------------------- *)
-val ring_symbols  : EcEnv.env -> ty -> (symbol * (bool * ty)) list
+val ring_symbols  : EcEnv.env -> bool -> ty -> (symbol * (bool * ty)) list
 val field_symbols : EcEnv.env -> ty -> (symbol * (bool * ty)) list
 
 val ring_axioms  : EcEnv.env -> ring  -> (symbol * form) list
