src/ecField.ml
@@ -11,79 +11,93 @@
 (* -------------------------------------------------------------------- *)
 open EcRing
 
-type fexpr =  FEc of c
-             | FEX of int
-             | FEadd of (fexpr * fexpr)
-             | FEsub of (fexpr * fexpr)
-             | FEmul of (fexpr * fexpr)
-             | FEopp of fexpr
-             | FEinv of fexpr
-             | FEdiv of (fexpr * fexpr)
-             | FEpow of (fexpr * int)
+type fexpr =  
+| FEc of c
+| FEX of int
+| FEadd of fexpr * fexpr
+| FEsub of fexpr * fexpr
+| FEmul of fexpr * fexpr
+| FEopp of fexpr
+| FEinv of fexpr
+| FEdiv of fexpr * fexpr
+| FEpow of fexpr * int
 
-type rsplit =  (pexpr * pexpr * pexpr)
+type rsplit = pexpr * pexpr * pexpr
 
 let left ((t,_,_) : rsplit) : pexpr = t
 let right ((_,_,t) : rsplit) : pexpr = t
 let common ((_,t,_) : rsplit) : pexpr = t
-
+  
 let npepow x n =
   match n with
-    | 0 -> PEc c1
-    | p -> if (p = 1) then x else
-               match x with
-                | PEc c -> if (ceq c c1) then PEc c1 else
-                            if (ceq c c0) then PEc c0 else 
-                              let res = Big_int.power_big_int_positive_int c p in
-                               PEc res 
-                | _ -> PEpow (x,n)
-
+  | 0 -> PEc c1
+  | p -> 
+    if p = 1 then x else
+      match x with
+      | PEc c -> 
+        if ceq c c1 then PEc c1 
+        else if ceq c c0 then PEc c0 
+        else 
+          let res = Big_int.power_big_int_positive_int c p in
+          PEc res 
+      | _ -> PEpow (x,n)
+        
 let rec npemul (x : pexpr) (y : pexpr) : pexpr =
-  match (x,y) with
-    | (PEc c, PEc c') -> PEc (cmul c c')
-    | (PEc c, _) -> if (ceq c c1) then y else if (ceq c c0) then PEc c0 else PEmul (x,y)
-    | (_,PEc c) -> if (ceq c c1) then x else if (ceq c c0) then PEc c0 else PEmul (x,y)
-    | (PEpow (e1,n1),PEpow (e2,n2)) -> if (n1 = n2) then npepow (npemul e1 e2) n1 else PEmul (x,y)
-    | (_,_) -> PEmul (x,y)
+  match x,y with
+  | PEc c, PEc c' -> PEc (cmul c c')
+  | PEc c, _ -> 
+    if ceq c c1 then y 
+    else if ceq c c0 then PEc c0 
+    else PEmul (x,y)
+  | _, PEc c -> 
+    if ceq c c1 then x 
+    else if ceq c c0 then PEc c0 
+    else PEmul (x,y)
+  | PEpow (e1,n1), PEpow (e2,n2) -> 
+    if n1 = n2 then npepow (npemul e1 e2) n1 
+    else PEmul (x,y)
+  | _,_ -> PEmul (x,y)
 
 let rec isIn (e1 : pexpr) (p1 : int) (e2 : pexpr) (p2 : int) : (int * pexpr) option =
   match e2 with
-    | PEmul (e3,e4) ->
-      (match (isIn e1 p1 e3 p2) with
-        | Some (0,e5) -> Some (0, npemul e5 (npepow e4 p2))                
-        | Some (p, e5) ->
-          (match (isIn e1 p e4 p2) with
-            | Some (n, e6) -> Some (n, npemul e5 e6)
-            | None -> Some (p, npemul e5 (npepow e4 p2)))
-        | None -> 
-          (match (isIn e1 p1 e4 p2) with
-            | Some (n,e5) -> Some (n,npemul (npepow e3 p2) e5)
-            | None -> None))
-          
-    | PEpow (_,0)   -> None
-    | PEpow (e3,p3) -> isIn e1 p1 e3 (p3 * p2)
-    | _ -> 
-      if (pexpr_eq e1 e2) then
-        if (p1 = p2) then Some (0, PEc c1) else
-          if (p1 > p2) then Some (p1-p2, PEc c1)
-            else Some (0, npepow e2 (p2-p1))
-      else None
+  | PEmul (e3,e4) ->
+    begin match isIn e1 p1 e3 p2 with
+    | Some (0,e5) -> Some (0, npemul e5 (npepow e4 p2))                
+    | Some (p, e5) ->
+      begin match isIn e1 p e4 p2 with
+      | Some (n, e6) -> Some (n, npemul e5 e6)
+      | None -> Some (p, npemul e5 (npepow e4 p2))
+      end
+    | None -> 
+      match isIn e1 p1 e4 p2 with
+      | Some (n,e5) -> Some (n,npemul (npepow e3 p2) e5)
+      | None -> None
+    end
+  | PEpow (_,0)   -> None
+  | PEpow (e3,p3) -> isIn e1 p1 e3 (p3 * p2)
+  | _ -> 
+    if pexpr_eq e1 e2 then
+      if p1 = p2 then Some (0, PEc c1) else
+        if p1 > p2 then Some (p1-p2, PEc c1)
+        else Some (0, npepow e2 (p2-p1))
+    else None
 
 let rec split_aux (e1 : pexpr) (p : int) (e2 : pexpr) : rsplit =
   match e1 with
-    | PEmul (e3,e4) ->
-      let r1 = split_aux e3 p e2 in
-      let r2 = split_aux e4 p (right r1) in
-        (npemul (left r1) (left r2),
-         npemul (common r1) (common r2),
-         right r2)
-    | PEpow (_,0) -> (PEc c1, PEc c1, e2)
-    | PEpow (e3,p3) -> split_aux e3 (p3 * p) e2
-    | _ ->
-          match isIn e1 p e2 1 with
-            | Some (0,e3) -> (PEc c1, npepow e1 p, e3)
-            | Some (q , e3) -> (npepow e1 q, npepow e1 (p - q), e3)
-            | None -> (npepow e1 p, PEc c1, e2)
+  | PEmul (e3,e4) ->
+    let r1 = split_aux e3 p e2 in
+    let r2 = split_aux e4 p (right r1) in
+    (npemul (left r1) (left r2),
+     npemul (common r1) (common r2),
+     right r2)
+  | PEpow (_,0) -> (PEc c1, PEc c1, e2)
+  | PEpow (e3,p3) -> split_aux e3 (p3 * p) e2
+  | _ ->
+    match isIn e1 p e2 1 with
+    | Some (0,e3) -> (PEc c1, npepow e1 p, e3)
+    | Some (q , e3) -> (npepow e1 q, npepow e1 (p - q), e3)
+    | None -> (npepow e1 p, PEc c1, e2)
+
 let split e1 e2 = split_aux e1 1 e2
 
 type linear = (pexpr * pexpr * (pexpr list))
@@ -93,63 +107,63 @@ let condition (_,_,t) = t
 
 let npeadd (e1 : pexpr) (e2 : pexpr) =
   match (e1,e2) with
-    | (PEc c, PEc c') -> PEc (cadd c c')
-    | (PEc c, _) -> if (ceq c c0) then e2 else PEadd (e1,e2)
-    | (_, PEc c) -> if (ceq c c0) then e1 else PEadd (e1,e2)
-    | _ -> PEadd (e1,e2)
+  | (PEc c, PEc c') -> PEc (cadd c c')
+  | (PEc c, _) -> if (ceq c c0) then e2 else PEadd (e1,e2)
+  | (_, PEc c) -> if (ceq c c0) then e1 else PEadd (e1,e2)
+  | _ -> PEadd (e1,e2)
 
 let npesub e1 e2 = 
   match (e1,e2) with
-    | (PEc c, PEc c') -> PEc (csub c c')
-    | (PEc c, _ ) -> if (ceq c c0) then PEopp e2 else PEsub (e1,e2)
-    | ( _, PEc c) -> if (ceq c c0) then e1 else PEsub (e1,e2)
-    | _ -> PEsub (e1,e2)
+  | (PEc c, PEc c') -> PEc (csub c c')
+  | (PEc c, _ ) -> if (ceq c c0) then PEopp e2 else PEsub (e1,e2)
+  | ( _, PEc c) -> if (ceq c c0) then e1 else PEsub (e1,e2)
+  | _ -> PEsub (e1,e2)
 
 let npeopp e1 =
   match e1 with
-    | PEc c -> PEc (copp c)
-    | _ -> PEopp e1
+  | PEc c -> PEc (copp c)
+  | _ -> PEopp e1
 
 let rec fnorm (e : fexpr) : linear =
   match e with
-    | FEc c -> (PEc c, PEc c1, [])
-    | FEX x -> (PEX x, PEc c1, [])
-    | FEadd (e1,e2) -> 
-      let x = fnorm e1 in
-      let y = fnorm e2 in
-      let s = split (denum x) (denum y) in
-      (npeadd (npemul (num x) (right s)) (npemul (num y) (left s)),
-      npemul (left s) (npemul (right s) (common s)),
-      condition x @ condition y)
-    | FEsub (e1,e2) ->
-      let x = fnorm e1 in
-      let y = fnorm e2 in
-      let s = split (denum x) (denum y) in
-      (npesub (npemul (num x) (right s)) (npemul (num y) (left s)),
-      npemul (left s) (npemul (right s) (common s)),
-      condition x @ condition y)
-    | FEmul (e1,e2) ->
-      let x = fnorm e1 in
-      let y = fnorm e2 in
-      let s1 = split (num x) (denum y) in
-      let s2 = split (num y) (denum x) in
-      (npemul (left s1) (left s2),
-      npemul (right s2) (right s1),
-      condition x @ condition y)
-    | FEopp e1 ->
-      let x = fnorm e1 in
-      (npeopp (num x), denum x, condition x)
-    | FEinv e ->
-      let x = fnorm e in
-      (denum x, num x, (num x) :: (condition x))
-    | FEdiv (e1,e2) -> 
-      let x = fnorm e1 in
-      let y = fnorm e2 in
-      let s1 = split (num x) (num y) in
-      let s2 = split (denum x) (denum y) in
-      (npemul (left s1) (right s2),
-      npemul (left s2) (right s1),
-      (num y) :: ((condition x) @ (condition y)))
-    | FEpow (e1,n) ->
-      let x = fnorm e1 in
-      (npepow (num x) n, npepow (denum x) n, condition x)
+  | FEc c -> (PEc c, PEc c1, [])
+  | FEX x -> (PEX x, PEc c1, [])
+  | FEadd (e1,e2) -> 
+    let x = fnorm e1 in
+    let y = fnorm e2 in
+    let s = split (denum x) (denum y) in
+    (npeadd (npemul (num x) (right s)) (npemul (num y) (left s)),
+     npemul (left s) (npemul (right s) (common s)),
+     condition x @ condition y)
+  | FEsub (e1,e2) ->
+    let x = fnorm e1 in
+    let y = fnorm e2 in
+    let s = split (denum x) (denum y) in
+    (npesub (npemul (num x) (right s)) (npemul (num y) (left s)),
+     npemul (left s) (npemul (right s) (common s)),
+     condition x @ condition y)
+  | FEmul (e1,e2) ->
+    let x = fnorm e1 in
+    let y = fnorm e2 in
+    let s1 = split (num x) (denum y) in
+    let s2 = split (num y) (denum x) in
+    (npemul (left s1) (left s2),
+     npemul (right s2) (right s1),
+     condition x @ condition y)
+  | FEopp e1 ->
+    let x = fnorm e1 in
+    (npeopp (num x), denum x, condition x)
+  | FEinv e ->
+    let x = fnorm e in
+    (denum x, num x, (num x) :: (condition x))
+  | FEdiv (e1,e2) -> 
+    let x = fnorm e1 in
+    let y = fnorm e2 in
+    let s1 = split (num x) (num y) in
+    let s2 = split (denum x) (denum y) in
+    (npemul (left s1) (right s2),
+     npemul (left s2) (right s1),
+     (num y) :: ((condition x) @ (condition y)))
+  | FEpow (e1,n) ->
+    let x = fnorm e1 in
+    (npepow (num x) n, npepow (denum x) n, condition x)
