src/ecField.mli
@@ -3,15 +3,15 @@ open EcRing
 
 (* -------------------------------------------------------------------- *)
 type fexpr =
-| FEc   of c
+| FEc   of Big_int.big_int
 | FEX   of int
-| FEadd of (fexpr * fexpr)
-| FEsub of (fexpr * fexpr)
-| FEmul of (fexpr * fexpr)
+| FEadd of fexpr * fexpr
+| FEsub of fexpr * fexpr
+| FEmul of fexpr * fexpr
 | FEopp of fexpr
 | FEinv of fexpr
-| FEdiv of (fexpr * fexpr)
-| FEpow of (fexpr * int)
+| FEdiv of fexpr * fexpr
+| FEpow of fexpr * int
 
 type linear = (pexpr * pexpr * (pexpr list))
 
