src/ecRing.ml
@@ -9,22 +9,11 @@
  *)
 
 (* -------------------------------------------------------------------- *)
+
 open Big_int
 
-type c = big_int
-
-let c0 = zero_big_int
-let c1 = unit_big_int
-
-let cadd a b = add_big_int a  b
-let csub a b = sub_big_int a  b
-let cmul a b = mult_big_int a  b
-let copp a =  minus_big_int a
-let ceq a b = eq_big_int a b
-let cdiv a b = quomod_big_int a b
-
 type pexpr = 
-  | PEc of c 
+  | PEc of big_int 
   | PEX of int
   | PEadd of pexpr * pexpr 
   | PEsub of pexpr * pexpr
@@ -40,319 +29,412 @@ let rec pp_pe fmt = function
   | PEmul(p1,p2) -> Format.fprintf fmt "%a * %a" pp_pe p1 pp_pe p2
   | PEopp p -> Format.fprintf fmt "-%a" pp_pe p
   | PEpow(p,i) -> Format.fprintf fmt "%a^%i" pp_pe p i
-  
-type pol =
-  | Pc of c 
-  | Pinj of int * pol
-  | PX of pol * int * pol
-
-let rec pp_pol fmt = function
-  | Pc c -> Format.fprintf fmt "%s" (string_of_big_int c)
-  | Pinj(i,p) -> Format.fprintf fmt "%i(%a)" i pp_pol p
-  | PX(q,i,p) -> Format.fprintf fmt "(%a^%i + %a)" pp_pol q i pp_pol p
-
-type mon = Mon0 | Zmon of (int * mon) | Vmon of (int * mon)
 
 let rec pexpr_eq (e1 : pexpr) (e2 : pexpr) : bool =
   match (e1,e2) with
-    | (PEc c, PEc c') -> ceq c c'
-    | (PEX p1, PEX p2) -> p1 = p2
-    | (PEadd (e3,e5), PEadd (e4,e6)) -> 
-      if (pexpr_eq e3 e4) then pexpr_eq e5 e6 else false
-    | (PEsub (e3,e5), PEsub (e4,e6)) -> 
-      if (pexpr_eq e3 e4) then pexpr_eq e5 e6 else false
-    | (PEmul (e3,e5), PEmul (e4,e6)) -> 
-      if (pexpr_eq e3 e4) then pexpr_eq e5 e6 else false
-    | (PEopp e3, PEopp e4) -> pexpr_eq e3 e4
-    | (PEpow (e3,n3), PEpow (e4,n4)) -> 
-      if (n3 = n4) then pexpr_eq e3 e4 else false
-    | (_,_) -> false
+  | (PEc c, PEc c') -> eq_big_int c c'
+  | (PEX p1, PEX p2) -> p1 = p2
+  | (PEadd (e3,e5), PEadd (e4,e6)) -> pexpr_eq e3 e4 && pexpr_eq e5 e6
+  | (PEsub (e3,e5), PEsub (e4,e6)) -> pexpr_eq e3 e4 && pexpr_eq e5 e6 
+  | (PEmul (e3,e5), PEmul (e4,e6)) -> pexpr_eq e3 e4 && pexpr_eq e5 e6 
+  | (PEopp e3, PEopp e4) -> pexpr_eq e3 e4
+  | (PEpow (e3,n3), PEpow (e4,n4)) -> n3 = n4 && pexpr_eq e3 e4 
+  | (_,_) -> false
 
-(**)
+type 'a cmp_sub = 
+  | Eq 
+  | Lt of 'a
+  | Gt of 'a
+ 
+module type Coef = sig
+  type c 
+  val cofint : big_int -> c
+  val ctoint : c -> big_int
+  val c0 : c
+  val c1 : c
+  val cadd : c -> c -> c
+  val csub : c -> c -> c
+  val cmul : c -> c -> c
+  val copp : c -> c 
+  val ceq  : c -> c -> bool
+  val cdiv : c -> c -> c*c
 
-let p0 = Pc c0
-let p1 = Pc c1
+  type p 
+  val pofint : int -> p
+  val ptoint : p -> int 
+  val padd : p -> p -> p
+  val peq  : p -> p -> bool
+  val pcmp : p -> p -> p cmp_sub
+    
+end
+ 
+module Cint = struct
+  type c = big_int
+  let cofint c = c
+  let ctoint c = c
+  let c0 = zero_big_int
+  let c1 = unit_big_int
 
-let mkXi i = PX (p1,i,p0) (* 1 * x_0 ^ i + 0  *)
+  let cadd a b = add_big_int a  b
+  let csub a b = sub_big_int a  b
+  let cmul a b = mult_big_int a  b
+  let copp a =  minus_big_int a
+  let ceq a b = eq_big_int a b
+  let cdiv a b = quomod_big_int a b
+    
+  type p = int
+  let pofint p = p
+  let ptoint p = p
+  let padd p1 p2 = p1 + p2
+  let peq (p1:p) p2 = p1 = p2
+  let pcmp p1 p2 = 
+    if p1 = p2 then Eq
+    else if p1 < p2 then Lt (p2 - p1)
+    else Gt (p1 - p2)
+    
+end
 
-let mkX = mkXi 1 (* ~= x ^ 1 *)
+module Cbool = struct
+  type c = int
 
-let mkPinj_pred j p = 
-  if (j=1) then p else Pinj(j-1,p)
+  let cofint c = 
+    int_of_big_int (and_big_int unit_big_int (abs_big_int c))
+  let ctoint c = big_int_of_int c
+    
+  let c0 = 0
+  let c1 = 1
 
-let mk_X j = mkPinj_pred j mkX
+  let cadd x y = x lxor y
+  let csub x y = x lxor y
+  let cmul x y = x land y
+  let copp x = x
+  let ceq (x:c) y = x = y
+  let cdiv x y = 
+    assert (y <> 0);
+    (x, 0)
 
-let rec peq (p : pol) (q:pol) : bool =
-  match (p,q) with
+  type p = unit
+
+  let pofint p = 
+    assert (1 <= p);
+    ()
+  let ptoint _p = 1
+
+  let padd _p1 _p2 = ()
+
+  let peq _p1 _p2 = true
+  let pcmp _p1 _p2 = Eq
+
+end
+
+module Make(C:Coef) = struct
+
+  module C = C
+  open C
+
+  type pol =
+  | Pc of c 
+  | Pinj of int * pol
+  | PX of pol * p * pol
+      
+  let rec pp_pol fmt = function
+    | Pc c -> Format.fprintf fmt "%s" (string_of_big_int (ctoint c))
+    | Pinj(i,p) -> 
+      Format.fprintf fmt "%i(%a)" i pp_pol p
+    | PX(q,i,p) -> 
+      Format.fprintf fmt "(%a^%i + %a)" pp_pol q (ptoint i) pp_pol p
+        
+  type mon = Mon0 | Zmon of (int * mon) | Vmon of (p * mon)
+     
+  let p0 = Pc c0
+  let p1 = Pc c1
+
+  let mkXi i = 
+    assert (1 <= i);
+    PX (p1,pofint i,p0) (* 1 * x_0 ^ i + 0  *)
+
+  let mkX = mkXi 1 (* ~= x ^ 1 *)
+
+  let mkPinj_pred j p = 
+    if j=1 then p else Pinj(j-1,p)
+      
+  let mk_X j = mkPinj_pred j mkX
+    
+  let rec peq (p : pol) (q:pol) : bool =
+    match (p,q) with
     | (Pc c1, Pc c2) -> ceq c1 c2
-    | (Pinj (j1,q1),Pinj (j2,q2)) -> if (j1 = j2) then peq q1 q2 else false
-    | (PX (p1,i1,q1), PX (p2,i2,q2)) -> if (i1 = i2) then
-                                            if (peq p1 p2) then
-                                                    peq q1 q2
-                                            else false
-                                        else false
+    | (Pinj (j1,q1),Pinj (j2,q2)) -> j1 = j2 && peq q1 q2
+    | (PX (p1,i1,q1), PX (p2,i2,q2)) -> C.peq i1 i2 && peq p1 p2 && peq q1 q2
     | _ -> false
 
-let mkPinj (j : int) (p : pol) : pol =
-	match p with
-		| Pc _ -> p
-		| Pinj (j',q) -> Pinj ((j+j'),q)
-		| _ -> Pinj (j,p)
+  let mkPinj (j : int) (p : pol) : pol =
+    match p with
+    | Pc _ -> p
+    | Pinj (j',q) -> Pinj ((j+j'),q)
+    | _ -> Pinj (j,p)
 
-let mkPX p i q =
-	match p with
-		| Pc c -> if (ceq c c0) then
-						mkPinj 1 q 
-					else PX (p,i,q)
-		| Pinj _ -> PX (p,i,q)
-		| PX (p',i',q') -> if (peq q' p0) then
-							PX (p',(i+i'),q)
-							else PX (p,i,q) 
+  let mkPX p i q =
+    match p with
+    | Pc c -> if ceq c c0 then mkPinj 1 q else PX(p,i,q)
+    | Pinj _ -> PX(p,i,q)
+    | PX (p',i',q') -> 
+      if peq q' p0 then PX (p',padd i i',q) else PX(p,i,q) 
 
-(* Opposite  *)
+  (* Opposite  *)
 
-let rec popp ( p : pol) : pol =
-  match p with
+  let rec popp ( p : pol) : pol =
+    match p with
     | Pc c -> Pc (copp c)
     | Pinj (j,q) -> Pinj (j, popp q)
     | PX (p,j,q) -> PX (popp p, j, popp q)
 
-(* Addition and Subs *)
+  (* Addition and Subs *)
 
-let rec paddc (p : pol) (c : c) : pol =
-  match p with
+  let rec paddc (p : pol) (c : c) : pol =
+    match p with
     | Pc c' -> Pc (cadd c' c)
     | Pinj (j,q) -> Pinj (j,paddc q c)
     | PX (p,j,q) -> PX (p,j, paddc q c)
 
-let rec psubc (p : pol) (c : c) : pol =
-  match p with
+  let rec psubc (p : pol) (c : c) : pol =
+    match p with
     | Pc c' -> Pc (csub c' c)
     | Pinj (j,q) -> Pinj (j,psubc q c)
     | PX (p,j,q) -> PX (p,j, psubc q c)
 
-let rec padd (p : pol) (p' : pol) : pol =
-  match p' with
+  let rec padd (p : pol) (p' : pol) : pol =
+    match p' with
     | Pc c -> paddc p c
     | Pinj (j',q') -> paddi q' j' p
-    | PX (p',i',q') ->  match p with
-                          | Pc c ->  PX (p',i',paddc q' c)
-                          | Pinj (j,q) -> if (j = 1) then
-                                            PX (p',i', padd q q') 
-                                          else
-                                            PX (p',i', padd (Pinj (j-1,q)) q')
-                          | PX (p,i,q) -> if (i = i') then
-                                            mkPX (padd p p') i (padd q q')
-                                          else if (i > i') then
-                                                mkPX (padd (PX (p,i-i',p0)) p') i' (padd q q')
-                                               else
-                                                mkPX (paddx p' (i'-i) p) i (padd q q')
-and paddi (q : pol) (j : int)  (p : pol) : pol =
-  match p with
-    | Pc c -> mkPinj j (paddc q c)
-    | Pinj (j',q') -> if (j' = j) then
-                        mkPinj j (padd q' q)
-                      else if (j' > j) then
-                            mkPinj j (padd (Pinj (j'-j,q')) q)
-                           else
-                            mkPinj j' (paddi q (j-j') q')
-    | PX (p,i,q') -> if (j = 1) then
-                        PX (p,i,padd q' q)
-                     else PX (p,i,paddi q (j-1) q')
-and paddx (p' : pol) (i' : int) (p : pol) : pol =
-  match p with
-    | Pc _ ->  PX (p',i',p)
-    | Pinj (j,q') -> if (j=1) then
-                      PX (p',i',q')
-                     else PX (p',i', Pinj (j-1,q'))
-    | PX (p,i,q') -> if (i=i') then
-                      mkPX (padd p p') i q'
-                     else if (i > i') then
-                            mkPX (padd (PX (p,(i-i'),p0)) p') i' q'
-                          else
-                            mkPX (paddx p' (i'-i) p) i q'
+    | PX (p',i',q') -> 
+      match p with
+      | Pc c ->  PX (p',i',paddc q' c)
+      | Pinj (j,q) -> 
+        if j = 1 then PX (p',i', padd q q') 
+        else PX(p',i', padd (Pinj (j-1,q)) q')
+      | PX (p,i,q) -> 
+        match pcmp i i' with
+        | Eq -> mkPX (padd p p') i (padd q q')
+        | Lt s -> mkPX (paddx p' s p) i (padd q q')
+        | Gt s -> mkPX (padd (PX (p,s,p0)) p') i' (padd q q')
 
-let rec psub (p : pol) (p' : pol) : pol =
-  match p' with
+  and paddi (q : pol) (j : int)  (p : pol) : pol =
+    match p with
+    | Pc c -> mkPinj j (paddc q c)
+    | Pinj (j',q') -> 
+      if j' = j then mkPinj j (padd q' q)
+      else if j' > j then mkPinj j (padd (Pinj (j'-j,q')) q)
+      else mkPinj j' (paddi q (j-j') q')
+    | PX (p,i,q') -> 
+      if j = 1 then PX (p,i,padd q' q)
+      else PX (p,i,paddi q (j-1) q')
+
+  and paddx (p' : pol) (i' : C.p) (p : pol) : pol =
+    match p with
+    | Pc _ ->  PX (p',i',p)
+    | Pinj (j,q') -> 
+      if j=1 then PX (p',i',q')
+      else PX (p',i', Pinj (j-1,q'))
+    | PX (p,i,q') -> 
+      match pcmp i i' with
+      | Eq -> mkPX (padd p p') i q'
+      | Gt s -> mkPX (padd (PX (p,s,p0)) p') i' q'
+      | Lt s -> mkPX (paddx p' s p) i q'
+
+  let rec psub (p : pol) (p' : pol) : pol =
+    match p' with
     | Pc c -> psubc p c
     | Pinj (j',q') -> psubi q' j' p
-    | PX (p',i',q') -> match p with
-                        | Pc c -> PX (popp p' , i', paddc (popp q') c)
-                        | Pinj (j,q) -> if (j=1) then
-                                          PX (popp p',i',psub q q') 
-                                        else PX (popp p',i', psub (Pinj (j-1,q)) q')
-                        | PX (p,i,q) -> if (i = i') then
-                                          mkPX  (psub p p') i (psub q q')
-                                        else if (i > i') then
-                                              mkPX (psub (PX (p,i-i',p0)) p') i' (psub q q')
-                                             else
-                                              mkPX (psubx p' (i'-i) p) i (psub q q')
-and psubi (q : pol) (j : int) ( p : pol) : pol =
-  match p with
-    | Pc c -> mkPinj j (paddc (popp q) c)
-    | Pinj (j',q') -> if ( j' = j ) then mkPinj j (psub q' q)
-                      else if (j' > j) then
-                              mkPinj j (psub (Pinj (j' - j,q')) q)   
-                           else
-                              mkPinj j' (psubi q (j-j') q')
-    | PX (p,i,q') -> if (j = 1) then
-                      PX (p,i,psub q' q) 
-                     else PX (p,i, psubi q (j-1) q')
-and psubx (p' : pol) (i' : int) (p : pol) : pol =
-  match p with
-    | Pc _ -> PX (popp p,i',p)
-    | Pinj (j,q') -> if (j = 1) then
-                       PX (popp p',i',q') 
-                     else PX (popp p',i', Pinj (j-1,q'))
-    | PX (p,i,q') -> if (i = i') then 
-                        mkPX (psub p p') i q'
-                     else if (i > i') then
-                             mkPX (psub (PX (p,i-i',p0)) p') i' q'
-                          else
-                             mkPX (psubx p' (i' -i)  p) i q'
+    | PX (p',i',q') -> 
+      match p with
+      | Pc c -> PX (popp p', i', paddc (popp q') c)
+      | Pinj (j,q) -> 
+        if j=1 then PX (popp p',i',psub q q') 
+        else PX (popp p',i', psub (Pinj (j-1,q)) q')
+      | PX (p,i,q) -> 
+        match pcmp i i' with
+        | Eq -> mkPX  (psub p p') i (psub q q')
+        | Gt s -> mkPX (psub (PX (p,s,p0)) p') i' (psub q q')
+        | Lt s -> mkPX (psubx p' s p) i (psub q q')
 
-let rec pmulc_aux (p : pol) (c : c) :pol =
-  match p with
+  and psubi (q : pol) (j : int) ( p : pol) : pol =
+    match p with
+    | Pc c -> mkPinj j (paddc (popp q) c)
+    | Pinj (j',q') -> 
+      if j' = j then mkPinj j (psub q' q)
+      else if j' > j then mkPinj j (psub (Pinj (j' - j,q')) q)   
+      else mkPinj j' (psubi q (j-j') q')
+    | PX (p,i,q') -> 
+      if j = 1 then PX (p,i,psub q' q) 
+      else PX (p,i, psubi q (j-1) q')
+
+  and psubx (p' : pol) (i' : C.p) (p : pol) : pol =
+    match p with
+    | Pc _ -> PX (popp p,i',p)
+    | Pinj (j,q') -> 
+      if j = 1 then PX (popp p',i',q') 
+      else PX (popp p',i', Pinj (j-1,q'))
+    | PX (p,i,q') -> 
+      match pcmp i i' with
+      | Eq -> mkPX (psub p p') i q'
+      | Gt s -> mkPX (psub (PX (p,s,p0)) p') i' q'
+      | Lt s -> mkPX (psubx p' s  p) i q'
+
+  let rec pmulc_aux (p : pol) (c : c) :pol =
+    match p with
     | Pc c' -> Pc (cmul c' c)
     | Pinj (j,q) -> mkPinj j (pmulc_aux q c)
     | PX (p,i,q) -> mkPX (pmulc_aux p c) i (pmulc_aux q c)
 
-let pmulc (p : pol) (c :c ) : pol =
-  if (ceq c c0) then p0 else if (ceq c c1) then p else pmulc_aux p c
+  let pmulc (p : pol) (c :c ) : pol =
+    if ceq c c0 then p0 
+    else if ceq c c1 then p else pmulc_aux p c
 
-let rec pmul (p : pol) (p'' : pol) : pol =
-  match p'' with
+  let rec pmul (p : pol) (p'' : pol) : pol =
+    match p'' with
     | Pc c -> pmulc p c
     | Pinj (j',q') -> pmuli q' j' p
-    | PX (p',i',q') -> match p with
-                        | Pc c -> pmulc p'' c
-                        | Pinj (j,q) -> let qq' = if (j = 1) then pmul q q' else pmul (Pinj (j-1,q)) q' in
-                          mkPX (pmul p p') i' qq'
-                        | PX (p,i,q) -> let qq' = pmul q q' in
-                                        let pq' = pmuli q' 1 p in
-                                        let qp' = pmul (mkPinj 1 q) p' in
-                                        let pp' = pmul p p' in
-                                        padd (mkPX (padd (mkPX pp' i p0) qp') i' p0) (mkPX pq' i qq')
-and pmuli (q : pol) (j : int) (p:pol) : pol =
-  match p with
+    | PX (p',i',q') -> 
+      match p with
+      | Pc c -> pmulc p'' c
+      | Pinj (j,q) -> 
+        let qq' = if j = 1 then pmul q q' else pmul (Pinj (j-1,q)) q' in
+        mkPX (pmul p p') i' qq'
+      | PX (p,i,q) -> 
+        let qq' = pmul q q' in
+        let pq' = pmuli q' 1 p in
+        let qp' = pmul (mkPinj 1 q) p' in
+        let pp' = pmul p p' in
+        padd (mkPX (padd (mkPX pp' i p0) qp') i' p0) (mkPX pq' i qq')
+
+  and pmuli (q : pol) (j : int) (p:pol) : pol =
+    match p with
     | Pc c -> mkPinj j (pmulc q c)
-    | Pinj (j',q') -> if (j' = j) then mkPinj j (pmul q' q) else
-                      if (j' > j) then mkPinj j (pmul (Pinj (j'-j,q')) q) else
-                                       mkPinj j' (pmuli q (j-j') q')
-    | PX (p',i',q') -> if (j = 1) then mkPX (pmuli q 1 p') i' (pmul q' q) else
-                       mkPX (pmuli q j p') i' (pmuli q (j-1) q')
+    | Pinj (j',q') -> 
+      if j' = j then mkPinj j (pmul q' q) 
+      else if j' > j then mkPinj j (pmul (Pinj (j'-j,q')) q) 
+      else mkPinj j' (pmuli q (j-j') q')
+    | PX (p',i',q') -> 
+      if j = 1 then mkPX (pmuli q 1 p') i' (pmul q' q) 
+      else mkPX (pmuli q j p') i' (pmuli q (j-1) q')
 
-let rec ppow_pos (res : pol) (p : pol) (t : int) : pol =
-  if (t = 1) then pmul res p else
-          ppow_pos (pmul res p) p (t-1)
-let rec ppow_n (p : pol) (n : int) : pol =
-  if (n = 0) then p1 else ppow_pos p1 p n
+  let rec ppow_pos (res : pol) (p : pol) (t : int) : pol =
+    if t = 1 then pmul res p 
+    else ppow_pos (pmul res p) p (t-1)
 
-(* Monomial *)
+  let rec ppow_n (p : pol) (n : int) : pol =
+    if (n = 0) then p1 else ppow_pos p1 p n
 
-let mkZmon j m =
-  match m with
+  let ppow_n (p:pol) (n:C.p) : pol =
+    ppow_n p (ptoint n)
+    
+  (* Monomial *)
+
+  let mkZmon j m =
+    match m with
     | Mon0 -> Mon0
     | Zmon(j',m) -> Zmon(j + j', m)
     | _ -> Zmon (j,m)
 
-let zmon_pred j m =
-  if (j = 1) then m else mkZmon (j-1) m
+  let zmon_pred j m =
+    if j = 1 then m else mkZmon (j-1) m
  
-let mkVmon i m =
-  match m with
+  let mkVmon i m =
+    match m with
     | Mon0 -> Vmon (i,Mon0)
-    | Zmon (j,m) -> Vmon (i,(zmon_pred j m))
-    | Vmon (i',m) -> Vmon ((i+i'),m)
+    | Zmon (j,m) -> Vmon (i,zmon_pred j m)
+    | Vmon (i',m) -> Vmon (C.padd i i',m)
 
-let rec cfactor (p : pol) ( c : c) : (pol * pol) =
-  match p with
+  let rec cfactor (p : pol) ( c : c) : (pol * pol) =
+    match p with
     | Pc c' ->
       let (q,r) = cdiv c' c in
-        (Pc r, Pc q) 
+      (Pc r, Pc q) 
     | Pinj (j1,p1) ->
       let (r,s) = cfactor p1 c in
-        (mkPinj j1 r, mkPinj j1 s)
+      (mkPinj j1 r, mkPinj j1 s)
     | PX (p1,i,q1) ->
       let (r1,s1) = cfactor p1 c in
       let (r2,s2) = cfactor q1 c in
-        (mkPX r1 i r2, mkPX s1 i s2)
+      (mkPX r1 i r2, mkPX s1 i s2)
 
-let rec mfactor (p : pol) (c : c) (m : mon) : pol * pol =
-  match (p,m) with
-    | (_, Mon0) -> if (ceq c c1) then (Pc c0, p) else cfactor p c
-    | (Pc _, _) -> (p, Pc c0)
-    | (Pinj (j1,p1), Zmon (j2,m1)) ->
-      if (j1 = j2) then
+  let rec mfactor (p : pol) (c : c) (m : mon) : pol * pol =
+    match p,m with
+    | _, Mon0 -> if (ceq c c1) then (Pc c0, p) else cfactor p c
+    | Pc _, _ -> (p, Pc c0)
+    | Pinj (j1,p1), Zmon (j2,m1) ->
+      if j1 = j2 then
         let (r,s) = mfactor p1 c m1 in
         (mkPinj j1 r, mkPinj j1 s)
-      else if (j1 < j2) then
+      else if j1 < j2 then
         let (r,s) = mfactor p1 c (Zmon ((j2-j1),m1)) in
         (mkPinj j1 r, mkPinj j1 s)
       else 
         (p, Pc c0)
-    | (Pinj _ , Vmon _) -> 
-      (p, Pc c0)
-    | (PX (p1,i,q1), Zmon (j,m1)) ->
+    | Pinj _ , Vmon _ -> 
+      p, Pc c0
+    | PX (p1,i,q1), Zmon (j,m1) ->
       let m2 = zmon_pred j m1 in
       let (r1,s1) = mfactor p1 c m in
       let (r2,s2) = mfactor q1 c m2 in
-        (mkPX r1 i r2, mkPX s1 i s2)
-    | (PX (p1,i,q1), Vmon (j,m1)) ->
-      if (i = j) then
+      (mkPX r1 i r2, mkPX s1 i s2)
+    | PX (p1,i,q1), Vmon (j,m1) ->
+      match pcmp i j with
+      | Eq -> 
         let (r1,s1) = mfactor p1 c (mkZmon 1 m1) in
         (mkPX r1 i q1, s1)
-      else if ( i < j) then
-        let (r1,s1) = mfactor p1 c (Vmon (j-i,m1)) in
+      | Lt s -> 
+        let (r1,s1) = mfactor p1 c (Vmon (s,m1)) in
         (mkPX r1 i q1, s1)
-      else
+      | Gt s ->
         let (r1,s1) = mfactor p1 c (mkZmon 1 m1) in
-        (mkPX r1 i q1, mkPX s1 (i-j) (Pc c0)) 
+        (mkPX r1 i q1, mkPX s1 s (Pc c0)) 
 
 
-let ponesubst (p1 : pol) ((c,m1) : c * mon) (p2 : pol) : pol option =    
-  let (q1,r1) = mfactor p1 c m1 in
-  match r1 with
+  let ponesubst (p1 : pol) ((c,m1) : c * mon) (p2 : pol) : pol option =    
+    let (q1,r1) = mfactor p1 c m1 in
+    match r1 with
     | Pc c -> 
-      if (ceq c c0) then None
+      if ceq c c0 then None
       else Some (padd q1 (pmul p2 r1))
     | _ -> 
       Some (padd q1 (pmul p2 r1))
-
-let rec pnsubstl (p1 : pol) (cm1 : c * mon) (p2 : pol) (n : int) : pol =
-  match (ponesubst p1 cm1 p2) with
+        
+  let rec pnsubstl (p1 : pol) (cm1 : c * mon) (p2 : pol) (n : int) : pol =
+    match ponesubst p1 cm1 p2 with
     | Some p3 -> 
-      if (n = 0) then p3 else
-                  pnsubstl p3 cm1 p2 (n-1)
+      if n = 0 then p3 else
+        pnsubstl p3 cm1 p2 (n-1)
     | _ -> p1
  
-let pnsubst (p1 : pol) (cm1 : c * mon) (p2 :pol) (n : int) : pol option =
-  match (ponesubst p1 cm1 p2) with
-    | Some p3 -> if (n = 0) then None
-                  else Some (pnsubstl p3 cm1 p2 (n-1))
+  let pnsubst (p1 : pol) (cm1 : c * mon) (p2 :pol) (n : int) : pol option =
+    match ponesubst p1 cm1 p2 with
+    | Some p3 -> 
+      if n = 0 then None
+      else Some (pnsubstl p3 cm1 p2 (n-1))
     | _ -> None
 
-let rec psubstl1 (p1 : pol) (lm1 : ((c * mon) * pol) list ) (n : int) : pol =
-  match lm1 with
+  let rec psubstl1 (p1 : pol) (lm1 : ((c * mon) * pol) list ) (n : int) : pol =
+    match lm1 with
     | [] -> p1
     | (m1,p2) :: lm2 -> psubstl1 (pnsubstl p1 m1 p2 n) lm2 n
 
-let rec psubstl (p1 : pol) (lm1 : ((c * mon) * pol) list) (n : int) : pol option =
-  match lm1 with
+  let rec psubstl (p1 : pol) (lm1 : ((c * mon) * pol) list) (n : int) : pol option =
+    match lm1 with
     | [] -> None
     | (m1,p2) :: lm2 -> 
       match pnsubst p1 m1 p2 n with
-        | Some p3 -> Some (psubstl1 p3 lm2 n)
-        | None -> psubstl p1 lm2 n
+      | Some p3 -> Some (psubstl1 p3 lm2 n)
+      | None -> psubstl p1 lm2 n
 
-let rec pnsubstl (p1 : pol) (lm1 : ((c * mon) * pol) list) (m : int) (n : int) : pol =
-  match psubstl p1 lm1 n with
-    | Some p3 -> if (m = 0) then p3 else pnsubstl p3 lm1 (m-1) n
+  let rec pnsubstl (p1 : pol) (lm1 : ((c * mon) * pol) list) (m : int) (n : int) : pol =
+    match psubstl p1 lm1 n with
+    | Some p3 -> if m = 0 then p3 else pnsubstl p3 lm1 (m-1) n
     | _ -> p1
  
-let rec norm_aux (e : pexpr) : pol =
-  match e with
-    | PEc c -> Pc c
+  let rec norm_aux (e : pexpr) : pol =
+    match e with
+    | PEc c -> Pc (cofint c)
     | PEX i -> mk_X i
     | PEadd (PEopp e1, e2) -> psub (norm_aux e2) (norm_aux e1) 
     | PEadd (e1, PEopp e2) -> psub (norm_aux e1) (norm_aux e2)
@@ -360,28 +442,74 @@ let rec norm_aux (e : pexpr) : pol =
     | PEmul (e1,e2) -> pmul (norm_aux e1) (norm_aux e2)
     | PEsub (e1,e2) -> psub (norm_aux e1) (norm_aux e2)
     | PEopp e1 -> popp (norm_aux e1)
-    | PEpow (e1,p) -> ppow_n (norm_aux e1) p 
+    | PEpow (e1,p) -> ppow_n (norm_aux e1) (pofint p) 
 
-let norm_subst (n : int) (lmp : ((c * mon) * pol) list) (p : pexpr) : pol  = 
-  pnsubstl (norm_aux p) lmp n n
+  let norm_subst (n : int) (lmp : ((c * mon) * pol) list) (p : pexpr) : pol  = 
+    pnsubstl (norm_aux p) lmp n n
 
 (* [mon_of_pol p = (c, m, r)] => p = c*m + r *)
-let rec mon_of_pol (p : pol) : (c * mon * pol) =
-  match p with
-  | Pc c -> c, Mon0, p0
-  | Pinj(j,p) ->
-    let c,m,r = mon_of_pol p in
-    c, mkZmon j m, mkPinj j r
-  | PX(p,i,q) ->
-    let c,m,r = mon_of_pol p in
-    c, mkVmon i m, mkPX r i q 
+  let rec mon_of_pol (p : pol) : (c * mon * pol) =
+    match p with
+    | Pc c -> c, Mon0, p0
+    | Pinj(j,p) ->
+      let c,m,r = mon_of_pol p in
+      c, mkZmon j m, mkPinj j r
+    | PX(p,i,q) ->
+      let c,m,r = mon_of_pol p in
+      c, mkVmon i m, mkPX r i q 
 
-let rec mk_monpol_list (lpe : (pexpr * pexpr) list) : ((c * mon) * pol) list =
-  match lpe with
+  let rec mk_monpol_list (lpe : (pexpr * pexpr) list) : ((c * mon) * pol) list =
+    match lpe with
     | [] -> []
     | (me,pe) :: lpe ->
       let c,m,r = mon_of_pol (norm_subst 0 [] me) in
       if ceq c c0 then mk_monpol_list lpe
       else ((c,m),psub (norm_subst 0 [] pe) r)::mk_monpol_list lpe
 
-let norm p lp = norm_subst 1000 (mk_monpol_list lp) p
+  let norm p lp = norm_subst 1000 (mk_monpol_list lp) p
+
+  let topexpr p = 
+    let rec doit idx = function
+      | Pc c -> PEc (ctoint c)
+      | Pinj (j, e) -> doit (idx+j) e
+      | PX (p, i, q) ->
+        let f = PEX idx in
+        let f = match ptoint i with 1 -> f | i -> PEpow(f, i) in
+        let f = if peq p p1 then f else PEmul(doit idx p, f) in
+        let f = if peq q p0 then f else PEadd(f, doit (idx+1) q) in
+        f
+    in
+    doit 1 p
+
+  let norm_pe p lp = topexpr (norm p lp)
+end
+
+module type Rnorm = sig
+
+  module C : Coef 
+    
+  type pol =
+  | Pc of C.c 
+  | Pinj of int * pol
+  | PX of pol * C.p * pol
+
+  val peq    : pol -> pol -> bool
+  val norm   : pexpr -> (pexpr * pexpr) list -> pol
+  val norm_pe: pexpr -> (pexpr * pexpr) list -> pexpr
+  val pp_pol : Format.formatter -> pol -> unit
+end
+
+module Iring = Make(Cint)
+module Bring = Make(Cbool)
+
+
+type c = big_int
+let c0 = zero_big_int
+let c1 = unit_big_int
+
+let cadd a b = add_big_int a  b
+let csub a b = sub_big_int a  b
+let cmul a b = mult_big_int a  b
+let copp a =  minus_big_int a
+let ceq a b = eq_big_int a b
+let cdiv a b = quomod_big_int a b
