src/ecRing.mli
@@ -1,20 +1,8 @@
+open Big_int
 (* -------------------------------------------------------------------- *)
-type c = Big_int.big_int
 
-val ceq : c -> c -> bool
-
-val c0 : c
-val c1 : c
-
-val cadd : c -> c -> c
-val csub : c -> c -> c
-val cmul : c -> c -> c
-val copp : c -> c
-val cdiv : c -> c -> c * c
-
-(* -------------------------------------------------------------------- *)
 type pexpr =
-| PEc   of c 
+| PEc   of big_int 
 | PEX   of int
 | PEadd of pexpr * pexpr 
 | PEsub of pexpr * pexpr
@@ -22,17 +10,68 @@ type pexpr =
 | PEopp of pexpr 
 | PEpow of pexpr * int
 
-type pol =
-| Pc of c 
-| Pinj of int * pol
-| PX of pol * int * pol
-
 val pexpr_eq : pexpr -> pexpr -> bool
-val peq : pol -> pol -> bool
-
-(* -------------------------------------------------------------------- *)
-val norm : pexpr -> (pexpr * pexpr) list -> pol
-
-(* -------------------------------------------------------------------- *)
 val pp_pe  : Format.formatter -> pexpr -> unit
-val pp_pol : Format.formatter -> pol   -> unit
+
+(* -------------------------------------------------------------------- *)
+
+type 'a cmp_sub = 
+  | Eq 
+  | Lt of 'a
+  | Gt of 'a
+
+module type Coef = sig
+  type c 
+  val cofint : big_int -> c
+  val ctoint : c -> big_int
+  val c0 : c
+  val c1 : c
+  val cadd : c -> c -> c
+  val csub : c -> c -> c
+  val cmul : c -> c -> c
+  val copp : c -> c 
+  val ceq  : c -> c -> bool
+  val cdiv : c -> c -> c*c
+
+  type p 
+  val pofint : int -> p
+  val ptoint : p -> int 
+  val padd : p -> p -> p
+  val peq  : p -> p -> bool
+  val pcmp : p -> p -> p cmp_sub
+
+end
+
+(* -------------------------------------------------------------------- *)
+module type Rnorm = sig
+
+  module C : Coef 
+    
+  type pol =
+  | Pc of C.c 
+  | Pinj of int * pol
+  | PX of pol * C.p * pol
+
+  val peq    : pol -> pol -> bool
+  val norm   : pexpr -> (pexpr * pexpr) list -> pol
+  val norm_pe: pexpr -> (pexpr * pexpr) list -> pexpr
+  val pp_pol : Format.formatter -> pol -> unit
+
+end
+
+module Iring : Rnorm
+module Bring : Rnorm
+
+(* -------------------------------------------------------------------- *)
+
+type c = big_int
+
+val c0 : c
+val c1 : c
+val cadd : c -> c -> c
+val csub : c -> c -> c
+val cmul : c -> c -> c
+val copp : c -> c 
+val ceq  : c -> c -> bool
+val cdiv : c -> c -> c*c
+
